lean/DMCFA.lean
@@ -21,3 +21,4 @@ import DMCFA.LNLemmas
 import DMCFA.LNSemantics
 import DMCFA.LNSoundness
 import DMCFA.LNSyntax
+import DMCFA.LNBridge
